src/coq/QC/GenMetadata.v
@@ -1,0 +1,1047 @@
+From Ltac2 Require Import Ltac2.
+From Coq Require Import List String.
+From Vellvm.Utils Require Import
+  IntMaps
+  Monads
+  Default.
+
+From Vellvm.Syntax Require Import
+  LLVMAst.
+
+From Vellvm.QC Require Import ECS Lens.
+Import LensNotations.
+Local Open Scope lens.
+
+Require Import ExtLib.Data.Monads.StateMonad.
+Require Import ExtLib.Data.Monads.OptionMonad.
+Require Import ExtLib.Data.Monads.ReaderMonad.
+Require Import ExtLib.Structures.Monads.
+Require Import ExtLib.Structures.Functor.
+Require Import ExtLib.Structures.Applicative.
+Require Import ExtLib.Structures.Traversable.
+Require Import ExtLib.Structures.Foldable.
+Require Import ExtLib.Structures.MonadPlus.
+Import MonadNotation.
+Import MonadPlusNotation.
+Import ApplicativeNotation.
+Import FunctorNotation.
+Import ListNotations.
+
+Record Metadata s :=
+  mkMetadata
+    { name : Component s Field ident
+    ; type_alias : Component s Field typ
+    ; variable_type : Component s Field typ
+    ; normalized_type : Component s Field typ
+    ; is_local : Component s Field unit
+    ; is_global : Component s Field unit
+    ; is_deterministic : Component s Field unit
+    ; is_non_deterministic : Component s Field unit
+    (* Whether the variable is the result of a pointer cast *)
+    ; from_pointer : Component s Field Ent
+    (* Whether the variable has a pointer type *)
+    ; is_pointer : Component s Field unit
+    (* Whether the variable is a pointer to sized type *)
+    ; is_sized_pointer : Component s Field unit
+    (* Whether the variable is of a sized type *)
+    ; is_sized : Component s Field unit
+    (* Whether the variable is an aggregate type *)
+    ; is_aggregate : Component s Field unit
+    (* Whether the variable is a vector type *)
+    ; is_vector : Component s Field unit
+    (* Whether the variable is an array type *)
+    ; is_array : Component s Field unit
+    (* Whether the variable is a structure type *)
+    ; is_struct : Component s Field unit
+    (* Whether the variable is a void type *)
+    ; is_non_void : Component s Field unit
+    (* Whether the variable is a pointer type or a vector of pointers *)
+    ; is_ptr_vector : Component s Field unit
+    (* Whether the variable is a pointer type or a vector of pointers to sized types *)
+    ; is_sized_ptr_vector : Component s Field unit
+    (* Whether a type alias is to a sized type *)
+    ; is_sized_type_alias : Component s Field unit
+    (* Whether a variable / type alias has a first class type *)
+    ; is_first_class_type : Component s Field unit
+    (* Whether a variable / type alias has a function pointer type *)
+    ; is_function_pointer : Component s Field unit
+    }.
+
+Definition blankSetter : (Metadata SetterOf).
+  constructor.
+  all: apply Keep.
+Defined.
+
+Definition defFields : (Metadata FieldOf).
+  constructor.
+  all: apply None.
+Defined.
+
+#[global] Instance Default_Metadata {s} : Default (Metadata s).
+split.
+destruct s.
+- apply defFields.
+- apply mkMetadata; apply IM.empty.
+- apply blankSetter.
+Defined.
+
+Ltac2 metadataConstructors :=
+  [ (fun _ => apply name)
+  ; (fun _ => apply type_alias)
+  ; (fun _ => apply variable_type)
+  ; (fun _ => apply normalized_type)
+  ; (fun _ => apply is_local)
+  ; (fun _ => apply is_global)
+  ; (fun _ => apply is_deterministic)
+  ; (fun _ => apply is_non_deterministic)
+  ; (fun _ => apply from_pointer)
+  ; (fun _ => apply is_pointer)
+  ; (fun _ => apply is_sized_pointer)
+  ; (fun _ => apply is_sized)
+  ; (fun _ => apply is_aggregate)
+  ; (fun _ => apply is_vector)
+  ; (fun _ => apply is_array)
+  ; (fun _ => apply is_struct)
+  ; (fun _ => apply is_non_void)
+  ; (fun _ => apply is_ptr_vector)
+  ; (fun _ => apply is_sized_ptr_vector)
+  ; (fun _ => apply is_sized_type_alias)
+  ; (fun _ => apply is_first_class_type)
+  ; (fun _ => apply is_function_pointer)
+  ].
+
+Ltac2 applyMetadataConstructors (tac : unit -> unit) :=
+  Control.dispatch
+    [ (fun _ => tac (); apply name)
+      ; (fun _ => tac (); apply type_alias)
+      ; (fun _ => tac (); apply variable_type)
+      ; (fun _ => tac (); apply normalized_type)
+      ; (fun _ => tac (); apply is_local)
+      ; (fun _ => tac (); apply is_global)
+      ; (fun _ => tac (); apply is_deterministic)
+      ; (fun _ => tac (); apply is_non_deterministic)
+      ; (fun _ => tac (); apply from_pointer)
+      ; (fun _ => tac (); apply is_pointer)
+      ; (fun _ => tac (); apply is_sized_pointer)
+      ; (fun _ => tac (); apply is_sized)
+      ; (fun _ => tac (); apply is_aggregate)
+      ; (fun _ => tac (); apply is_vector)
+      ; (fun _ => tac (); apply is_array)
+      ; (fun _ => tac (); apply is_struct)
+      ; (fun _ => tac (); apply is_non_void)
+      ; (fun _ => tac (); apply is_ptr_vector)
+      ; (fun _ => tac (); apply is_sized_ptr_vector)
+      ; (fun _ => tac (); apply is_sized_type_alias)
+      ; (fun _ => tac (); apply is_first_class_type)
+      ; (fun _ => tac (); apply is_function_pointer)
+    ].
+
+Definition getEntity {w m} `{Monad m} `{@MetadataStore m Metadata (SystemState w m)}
+  (entity : Ent) : SystemT w m (Metadata FieldOf).
+  refine open_constr:(let entity_id := unEnt entity in
+                      storage <- use metadata;;
+                      ret (_)); try typeclasses_eauto.
+  apply (mkMetadata FieldOf);
+    refine open_constr:(IM.Raw.find entity_id (_ storage));
+    Control.dispatch metadataConstructors.
+Defined.
+
+Definition setterOfFields (vals : Metadata FieldOf) : Metadata SetterOf.
+  constructor;
+    applyMetadataConstructors (fun _ => refine open_constr:(optionToUpdate (_ vals))).
+Defined.
+
+Definition setEntity
+  {w m} `{Monad m} `{@MetadataStore m Metadata (SystemState w m)}
+  (entity : Ent) (setter : Metadata SetterOf) : SystemT w m unit.
+  refine
+    open_constr:(let entity_id := unEnt entity in
+                 metadata _ _ %= (fun storage => _);;
+                 entities %= (fun ents => IS.add entity_id ents);;
+                 ret tt);
+    try typeclasses_eauto.
+  apply (mkMetadata (WorldOf m));
+    applyMetadataConstructors (fun _ => refine open_constr:(updateIntMapRaw (_ setter) entity_id (_ storage))).
+Defined.
+
+Definition setEntities
+  {w : StorageType -> Type} {m : Type -> Type}
+  `{Monad m} `{@MetadataStore m Metadata (SystemState w m)}
+  (es : IM.Raw.t (Metadata FieldOf)) : SystemT w m unit
+  := IM.Raw.fold (fun k fs acc => setEntity (mkEnt k) (setterOfFields fs);; acc) es (ret tt).
+
+Definition name' {s : StorageType} : Lens' (Metadata s) (Component s Field ident).
+  red.
+  intros f F afa w.
+  refine open_constr:((fun x => _) <$> afa (_ w)); try typeclasses_eauto.
+  - apply mkMetadata;
+      Control.dispatch
+        [ (fun _ => apply x)
+          ; (fun _ => apply type_alias)
+          ; (fun _ => apply variable_type)
+          ; (fun _ => apply normalized_type)
+          ; (fun _ => apply is_local)
+          ; (fun _ => apply is_global)
+          ; (fun _ => apply is_deterministic)
+          ; (fun _ => apply is_non_deterministic)
+          ; (fun _ => apply from_pointer)
+          ; (fun _ => apply is_pointer)
+          ; (fun _ => apply is_sized_pointer)
+          ; (fun _ => apply is_sized)
+          ; (fun _ => apply is_aggregate)
+          ; (fun _ => apply is_vector)
+          ; (fun _ => apply is_array)
+          ; (fun _ => apply is_struct)
+          ; (fun _ => apply is_non_void)
+          ; (fun _ => apply is_ptr_vector)
+          ; (fun _ => apply is_sized_ptr_vector)
+          ; (fun _ => apply is_sized_type_alias)
+          ; (fun _ => apply is_first_class_type)
+          ; (fun _ => apply is_function_pointer)
+        ];
+      apply w.
+  - apply name.
+Defined.
+
+Definition is_global' {s : StorageType} : Lens' (Metadata s) (Component s Field unit).
+  red.
+  intros f F afa w.
+  refine open_constr:((fun x => _) <$> afa (_ w)); try typeclasses_eauto.
+  - apply mkMetadata;
+      Control.dispatch
+        [ (fun _ => apply name)
+          ; (fun _ => apply type_alias)
+          ; (fun _ => apply variable_type)
+          ; (fun _ => apply normalized_type)
+          ; (fun _ => apply is_local)
+          ; (fun _ => apply x)
+          ; (fun _ => apply is_deterministic)
+          ; (fun _ => apply is_non_deterministic)
+          ; (fun _ => apply from_pointer)
+          ; (fun _ => apply is_pointer)
+          ; (fun _ => apply is_sized_pointer)
+          ; (fun _ => apply is_sized)
+          ; (fun _ => apply is_aggregate)
+          ; (fun _ => apply is_vector)
+          ; (fun _ => apply is_array)
+          ; (fun _ => apply is_struct)
+          ; (fun _ => apply is_non_void)
+          ; (fun _ => apply is_ptr_vector)
+          ; (fun _ => apply is_sized_ptr_vector)
+          ; (fun _ => apply is_sized_type_alias)
+          ; (fun _ => apply is_first_class_type)
+          ; (fun _ => apply is_function_pointer)
+        ];
+      apply w.
+  - apply is_global.
+Defined.
+
+Definition is_local' {s : StorageType} : Lens' (Metadata s) (Component s Field unit).
+  red.
+  intros f F afa w.
+  refine open_constr:((fun x => _) <$> afa (_ w)); try typeclasses_eauto.
+  - apply mkMetadata;
+      Control.dispatch
+        [ (fun _ => apply name)
+          ; (fun _ => apply type_alias)
+          ; (fun _ => apply variable_type)
+          ; (fun _ => apply normalized_type)
+          ; (fun _ => apply x)
+          ; (fun _ => apply is_global)
+          ; (fun _ => apply is_deterministic)
+          ; (fun _ => apply is_non_deterministic)
+          ; (fun _ => apply from_pointer)
+          ; (fun _ => apply is_pointer)
+          ; (fun _ => apply is_sized_pointer)
+          ; (fun _ => apply is_sized)
+          ; (fun _ => apply is_aggregate)
+          ; (fun _ => apply is_vector)
+          ; (fun _ => apply is_array)
+          ; (fun _ => apply is_struct)
+          ; (fun _ => apply is_non_void)
+          ; (fun _ => apply is_ptr_vector)
+          ; (fun _ => apply is_sized_ptr_vector)
+          ; (fun _ => apply is_sized_type_alias)
+          ; (fun _ => apply is_first_class_type)
+          ; (fun _ => apply is_function_pointer)
+        ];
+      apply w.
+  - apply is_local.
+Defined.
+
+Definition type_alias' {s : StorageType} : Lens' (Metadata s) (Component s Field typ).
+  red.
+  intros f F afa w.
+  refine open_constr:((fun x => _) <$> afa (_ w)); try typeclasses_eauto.
+  - apply mkMetadata;
+      Control.dispatch
+        [ (fun _ => apply name)
+          ; (fun _ => apply x)
+          ; (fun _ => apply variable_type)
+          ; (fun _ => apply normalized_type)
+          ; (fun _ => apply is_local)
+          ; (fun _ => apply is_global)
+          ; (fun _ => apply is_deterministic)
+          ; (fun _ => apply is_non_deterministic)
+          ; (fun _ => apply from_pointer)
+          ; (fun _ => apply is_pointer)
+          ; (fun _ => apply is_sized_pointer)
+          ; (fun _ => apply is_sized)
+          ; (fun _ => apply is_aggregate)
+          ; (fun _ => apply is_vector)
+          ; (fun _ => apply is_array)
+          ; (fun _ => apply is_struct)
+          ; (fun _ => apply is_non_void)
+          ; (fun _ => apply is_ptr_vector)
+          ; (fun _ => apply is_sized_ptr_vector)
+          ; (fun _ => apply is_sized_type_alias)
+          ; (fun _ => apply is_first_class_type)
+          ; (fun _ => apply is_function_pointer)
+        ];
+      apply w.
+  - apply type_alias.
+Defined.
+
+Definition variable_type' {s : StorageType} : Lens' (Metadata s) (Component s Field typ).
+  red.
+  intros f F afa w.
+  refine open_constr:((fun x => _) <$> afa (_ w)); try typeclasses_eauto.
+  - apply mkMetadata;
+      Control.dispatch
+        [ (fun _ => apply name)
+          ; (fun _ => apply type_alias)
+          ; (fun _ => apply x)
+          ; (fun _ => apply normalized_type)
+          ; (fun _ => apply is_local)
+          ; (fun _ => apply is_global)
+          ; (fun _ => apply is_deterministic)
+          ; (fun _ => apply is_non_deterministic)
+          ; (fun _ => apply from_pointer)
+          ; (fun _ => apply is_pointer)
+          ; (fun _ => apply is_sized_pointer)
+          ; (fun _ => apply is_sized)
+          ; (fun _ => apply is_aggregate)
+          ; (fun _ => apply is_vector)
+          ; (fun _ => apply is_array)
+          ; (fun _ => apply is_struct)
+          ; (fun _ => apply is_non_void)
+          ; (fun _ => apply is_ptr_vector)
+          ; (fun _ => apply is_sized_ptr_vector)
+          ; (fun _ => apply is_sized_type_alias)
+          ; (fun _ => apply is_first_class_type)
+          ; (fun _ => apply is_function_pointer)
+        ];
+      apply w.
+  - apply variable_type.
+Defined.
+
+Definition normalized_type' {s : StorageType} : Lens' (Metadata s) (Component s Field typ).
+  red.
+  intros f F afa w.
+  refine open_constr:((fun x => _) <$> afa (_ w)); try typeclasses_eauto.
+  - apply mkMetadata;
+      Control.dispatch
+        [ (fun _ => apply name)
+          ; (fun _ => apply type_alias)
+          ; (fun _ => apply variable_type)
+          ; (fun _ => apply x)
+          ; (fun _ => apply is_local)
+          ; (fun _ => apply is_global)
+          ; (fun _ => apply is_deterministic)
+          ; (fun _ => apply is_non_deterministic)
+          ; (fun _ => apply from_pointer)
+          ; (fun _ => apply is_pointer)
+          ; (fun _ => apply is_sized_pointer)
+          ; (fun _ => apply is_sized)
+          ; (fun _ => apply is_aggregate)
+          ; (fun _ => apply is_vector)
+          ; (fun _ => apply is_array)
+          ; (fun _ => apply is_struct)
+          ; (fun _ => apply is_non_void)
+          ; (fun _ => apply is_ptr_vector)
+          ; (fun _ => apply is_sized_ptr_vector)
+          ; (fun _ => apply is_sized_type_alias)
+          ; (fun _ => apply is_first_class_type)
+          ; (fun _ => apply is_function_pointer)
+        ];
+      apply w.
+  - apply normalized_type.
+Defined.
+
+Definition is_deterministic' {s : StorageType} : Lens' (Metadata s) (Component s Field unit).
+  red.
+  intros f F afa w.
+  refine open_constr:((fun x => _) <$> afa (_ w)); try typeclasses_eauto.
+  - apply mkMetadata;
+      Control.dispatch
+        [ (fun _ => apply name)
+          ; (fun _ => apply type_alias)
+          ; (fun _ => apply variable_type)
+          ; (fun _ => apply normalized_type)
+          ; (fun _ => apply is_local)
+          ; (fun _ => apply is_global)
+          ; (fun _ => apply x)
+          ; (fun _ => apply is_non_deterministic)
+          ; (fun _ => apply from_pointer)
+          ; (fun _ => apply is_pointer)
+          ; (fun _ => apply is_sized_pointer)
+          ; (fun _ => apply is_sized)
+          ; (fun _ => apply is_aggregate)
+          ; (fun _ => apply is_vector)
+          ; (fun _ => apply is_array)
+          ; (fun _ => apply is_struct)
+          ; (fun _ => apply is_non_void)
+          ; (fun _ => apply is_ptr_vector)
+          ; (fun _ => apply is_sized_ptr_vector)
+          ; (fun _ => apply is_sized_type_alias)
+          ; (fun _ => apply is_first_class_type)
+          ; (fun _ => apply is_function_pointer)
+        ];
+      apply w.
+  - apply is_deterministic.
+Defined.
+
+Definition is_non_deterministic' {s : StorageType} : Lens' (Metadata s) (Component s Field unit).
+  red.
+  intros f F afa w.
+  refine open_constr:((fun x => _) <$> afa (_ w)); try typeclasses_eauto.
+  - apply mkMetadata;
+      Control.dispatch
+        [ (fun _ => apply name)
+          ; (fun _ => apply type_alias)
+          ; (fun _ => apply variable_type)
+          ; (fun _ => apply normalized_type)
+          ; (fun _ => apply is_local)
+          ; (fun _ => apply is_global)
+          ; (fun _ => apply is_deterministic)
+          ; (fun _ => apply x)
+          ; (fun _ => apply from_pointer)
+          ; (fun _ => apply is_pointer)
+          ; (fun _ => apply is_sized_pointer)
+          ; (fun _ => apply is_sized)
+          ; (fun _ => apply is_aggregate)
+          ; (fun _ => apply is_vector)
+          ; (fun _ => apply is_array)
+          ; (fun _ => apply is_struct)
+          ; (fun _ => apply is_non_void)
+          ; (fun _ => apply is_ptr_vector)
+          ; (fun _ => apply is_sized_ptr_vector)
+          ; (fun _ => apply is_sized_type_alias)
+          ; (fun _ => apply is_first_class_type)
+          ; (fun _ => apply is_function_pointer)
+        ];
+      apply w.
+  - apply is_non_deterministic.
+Defined.
+
+Definition invert_option_unit (x : option unit) : option unit
+  := match x with
+     | Some _ => None
+     | None => Some tt
+     end.
+
+Definition deterministic' : Lens' (Metadata FieldOf) bool.
+  red.
+  intros F HF f fields.
+  ltac1:(pose proof (is_some (fields .^ is_deterministic')) as deterministicb).
+  apply f in deterministicb.
+  apply (fmap
+           (fun (b : bool) =>
+              if b
+              then (fields
+                    & @is_deterministic' FieldOf .~ ret tt
+                    & @is_non_deterministic' FieldOf .~ None)
+              else (fields
+                    & @is_deterministic' FieldOf .~ None
+                    & @is_non_deterministic' FieldOf .~ ret tt))).
+  apply deterministicb.
+Defined.
+
+Definition from_pointer' {s : StorageType} : Lens' (Metadata s) (Component s Field Ent).
+  red.
+  intros f F afa w.
+  refine open_constr:((fun x => _) <$> afa (_ w)); try typeclasses_eauto.
+  - apply mkMetadata;
+      Control.dispatch
+        [ (fun _ => apply name)
+          ; (fun _ => apply type_alias)
+          ; (fun _ => apply variable_type)
+          ; (fun _ => apply normalized_type)
+          ; (fun _ => apply is_local)
+          ; (fun _ => apply is_global)
+          ; (fun _ => apply is_deterministic)
+          ; (fun _ => apply is_non_deterministic)
+          ; (fun _ => apply x)
+          ; (fun _ => apply is_pointer)
+          ; (fun _ => apply is_sized_pointer)
+          ; (fun _ => apply is_sized)
+          ; (fun _ => apply is_aggregate)
+          ; (fun _ => apply is_vector)
+          ; (fun _ => apply is_array)
+          ; (fun _ => apply is_struct)
+          ; (fun _ => apply is_non_void)
+          ; (fun _ => apply is_ptr_vector)
+          ; (fun _ => apply is_sized_ptr_vector)
+          ; (fun _ => apply is_sized_type_alias)
+          ; (fun _ => apply is_first_class_type)
+          ; (fun _ => apply is_function_pointer)
+        ];
+      apply w.
+  - apply from_pointer.
+Defined.
+
+Definition is_pointer' {s : StorageType} : Lens' (Metadata s) (Component s Field unit).
+  red.
+  intros f F afa w.
+  refine open_constr:((fun x => _) <$> afa (_ w)); try typeclasses_eauto.
+  - apply mkMetadata;
+      Control.dispatch
+        [ (fun _ => apply name)
+          ; (fun _ => apply type_alias)
+          ; (fun _ => apply variable_type)
+          ; (fun _ => apply normalized_type)
+          ; (fun _ => apply is_local)
+          ; (fun _ => apply is_global)
+          ; (fun _ => apply is_deterministic)
+          ; (fun _ => apply is_non_deterministic)
+          ; (fun _ => apply from_pointer)
+          ; (fun _ => apply x)
+          ; (fun _ => apply is_sized_pointer)
+          ; (fun _ => apply is_sized)
+          ; (fun _ => apply is_aggregate)
+          ; (fun _ => apply is_vector)
+          ; (fun _ => apply is_array)
+          ; (fun _ => apply is_struct)
+          ; (fun _ => apply is_non_void)
+          ; (fun _ => apply is_ptr_vector)
+          ; (fun _ => apply is_sized_ptr_vector)
+          ; (fun _ => apply is_sized_type_alias)
+          ; (fun _ => apply is_first_class_type)
+          ; (fun _ => apply is_function_pointer)
+        ];
+      apply w.
+  - apply is_pointer.
+Defined.
+
+Definition is_sized_pointer' {s : StorageType} : Lens' (Metadata s) (Component s Field unit).
+  red.
+  intros f F afa w.
+  refine open_constr:((fun x => _) <$> afa (_ w)); try typeclasses_eauto.
+  - apply mkMetadata;
+      Control.dispatch
+        [ (fun _ => apply name)
+          ; (fun _ => apply type_alias)
+          ; (fun _ => apply variable_type)
+          ; (fun _ => apply normalized_type)
+          ; (fun _ => apply is_local)
+          ; (fun _ => apply is_global)
+          ; (fun _ => apply is_deterministic)
+          ; (fun _ => apply is_non_deterministic)
+          ; (fun _ => apply from_pointer)
+          ; (fun _ => apply is_pointer)
+          ; (fun _ => apply x)
+          ; (fun _ => apply is_sized)
+          ; (fun _ => apply is_aggregate)
+          ; (fun _ => apply is_vector)
+          ; (fun _ => apply is_array)
+          ; (fun _ => apply is_struct)
+          ; (fun _ => apply is_non_void)
+          ; (fun _ => apply is_ptr_vector)
+          ; (fun _ => apply is_sized_ptr_vector)
+          ; (fun _ => apply is_sized_type_alias)
+          ; (fun _ => apply is_first_class_type)
+          ; (fun _ => apply is_function_pointer)
+        ];
+      apply w.
+  - apply is_sized_pointer.
+Defined.
+
+Definition is_sized' {s : StorageType} : Lens' (Metadata s) (Component s Field unit).
+  red.
+  intros f F afa w.
+  refine open_constr:((fun x => _) <$> afa (_ w)); try typeclasses_eauto.
+  - apply mkMetadata;
+      Control.dispatch
+        [ (fun _ => apply name)
+          ; (fun _ => apply type_alias)
+          ; (fun _ => apply variable_type)
+          ; (fun _ => apply normalized_type)
+          ; (fun _ => apply is_local)
+          ; (fun _ => apply is_global)
+          ; (fun _ => apply is_deterministic)
+          ; (fun _ => apply is_non_deterministic)
+          ; (fun _ => apply from_pointer)
+          ; (fun _ => apply is_pointer)
+          ; (fun _ => apply is_sized_pointer)
+          ; (fun _ => apply x)
+          ; (fun _ => apply is_aggregate)
+          ; (fun _ => apply is_vector)
+          ; (fun _ => apply is_array)
+          ; (fun _ => apply is_struct)
+          ; (fun _ => apply is_non_void)
+          ; (fun _ => apply is_ptr_vector)
+          ; (fun _ => apply is_sized_ptr_vector)
+          ; (fun _ => apply is_sized_type_alias)
+          ; (fun _ => apply is_first_class_type)
+          ; (fun _ => apply is_function_pointer)
+        ];
+      apply w.
+  - apply is_sized.
+Defined.
+
+Definition is_aggregate' {s : StorageType} : Lens' (Metadata s) (Component s Field unit).
+  red.
+  intros f F afa w.
+  refine open_constr:((fun x => _) <$> afa (_ w)); try typeclasses_eauto.
+  - apply mkMetadata;
+      Control.dispatch
+        [ (fun _ => apply name)
+          ; (fun _ => apply type_alias)
+          ; (fun _ => apply variable_type)
+          ; (fun _ => apply normalized_type)
+          ; (fun _ => apply is_local)
+          ; (fun _ => apply is_global)
+          ; (fun _ => apply is_deterministic)
+          ; (fun _ => apply is_non_deterministic)
+          ; (fun _ => apply from_pointer)
+          ; (fun _ => apply is_pointer)
+          ; (fun _ => apply is_sized_pointer)
+          ; (fun _ => apply is_sized)
+          ; (fun _ => apply x)
+          ; (fun _ => apply is_vector)
+          ; (fun _ => apply is_array)
+          ; (fun _ => apply is_struct)
+          ; (fun _ => apply is_non_void)
+          ; (fun _ => apply is_ptr_vector)
+          ; (fun _ => apply is_sized_ptr_vector)
+          ; (fun _ => apply is_sized_type_alias)
+          ; (fun _ => apply is_first_class_type)
+          ; (fun _ => apply is_function_pointer)
+        ];
+      apply w.
+  - apply is_aggregate.
+Defined.
+
+Definition is_vector' {s : StorageType} : Lens' (Metadata s) (Component s Field unit).
+  red.
+  intros f F afa w.
+  refine open_constr:((fun x => _) <$> afa (_ w)); try typeclasses_eauto.
+  - apply mkMetadata;
+      Control.dispatch
+        [ (fun _ => apply name)
+          ; (fun _ => apply type_alias)
+          ; (fun _ => apply variable_type)
+          ; (fun _ => apply normalized_type)
+          ; (fun _ => apply is_local)
+          ; (fun _ => apply is_global)
+          ; (fun _ => apply is_deterministic)
+          ; (fun _ => apply is_non_deterministic)
+          ; (fun _ => apply from_pointer)
+          ; (fun _ => apply is_pointer)
+          ; (fun _ => apply is_sized_pointer)
+          ; (fun _ => apply is_sized)
+          ; (fun _ => apply is_aggregate)
+          ; (fun _ => apply x)
+          ; (fun _ => apply is_array)
+          ; (fun _ => apply is_struct)
+          ; (fun _ => apply is_non_void)
+          ; (fun _ => apply is_ptr_vector)
+          ; (fun _ => apply is_sized_ptr_vector)
+          ; (fun _ => apply is_sized_type_alias)
+          ; (fun _ => apply is_first_class_type)
+          ; (fun _ => apply is_function_pointer)
+        ];
+      apply w.
+  - apply is_vector.
+Defined.
+
+Definition is_array' {s : StorageType} : Lens' (Metadata s) (Component s Field unit).
+  red.
+  intros f F afa w.
+  refine open_constr:((fun x => _) <$> afa (_ w)); try typeclasses_eauto.
+  - apply mkMetadata;
+      Control.dispatch
+        [ (fun _ => apply name)
+          ; (fun _ => apply type_alias)
+          ; (fun _ => apply variable_type)
+          ; (fun _ => apply normalized_type)
+          ; (fun _ => apply is_local)
+          ; (fun _ => apply is_global)
+          ; (fun _ => apply is_deterministic)
+          ; (fun _ => apply is_non_deterministic)
+          ; (fun _ => apply from_pointer)
+          ; (fun _ => apply is_pointer)
+          ; (fun _ => apply is_sized_pointer)
+          ; (fun _ => apply is_sized)
+          ; (fun _ => apply is_aggregate)
+          ; (fun _ => apply is_vector)
+          ; (fun _ => apply x)
+          ; (fun _ => apply is_struct)
+          ; (fun _ => apply is_non_void)
+          ; (fun _ => apply is_ptr_vector)
+          ; (fun _ => apply is_sized_ptr_vector)
+          ; (fun _ => apply is_sized_type_alias)
+          ; (fun _ => apply is_first_class_type)
+          ; (fun _ => apply is_function_pointer)
+        ];
+      apply w.
+  - apply is_array.
+Defined.
+
+Definition is_struct' {s : StorageType} : Lens' (Metadata s) (Component s Field unit).
+  red.
+  intros f F afa w.
+  refine open_constr:((fun x => _) <$> afa (_ w)); try typeclasses_eauto.
+  - apply mkMetadata;
+      Control.dispatch
+        [ (fun _ => apply name)
+          ; (fun _ => apply type_alias)
+          ; (fun _ => apply variable_type)
+          ; (fun _ => apply normalized_type)
+          ; (fun _ => apply is_local)
+          ; (fun _ => apply is_global)
+          ; (fun _ => apply is_deterministic)
+          ; (fun _ => apply is_non_deterministic)
+          ; (fun _ => apply from_pointer)
+          ; (fun _ => apply is_pointer)
+          ; (fun _ => apply is_sized_pointer)
+          ; (fun _ => apply is_sized)
+          ; (fun _ => apply is_aggregate)
+          ; (fun _ => apply is_vector)
+          ; (fun _ => apply is_array)
+          ; (fun _ => apply x)
+          ; (fun _ => apply is_non_void)
+          ; (fun _ => apply is_ptr_vector)
+          ; (fun _ => apply is_sized_ptr_vector)
+          ; (fun _ => apply is_sized_type_alias)
+          ; (fun _ => apply is_first_class_type)
+          ; (fun _ => apply is_function_pointer)
+        ];
+      apply w.
+  - apply is_struct.
+Defined.
+
+Definition is_non_void' {s : StorageType} : Lens' (Metadata s) (Component s Field unit).
+  red.
+  intros f F afa w.
+  refine open_constr:((fun x => _) <$> afa (_ w)); try typeclasses_eauto.
+  - apply mkMetadata;
+      Control.dispatch
+        [ (fun _ => apply name)
+          ; (fun _ => apply type_alias)
+          ; (fun _ => apply variable_type)
+          ; (fun _ => apply normalized_type)
+          ; (fun _ => apply is_local)
+          ; (fun _ => apply is_global)
+          ; (fun _ => apply is_deterministic)
+          ; (fun _ => apply is_non_deterministic)
+          ; (fun _ => apply from_pointer)
+          ; (fun _ => apply is_pointer)
+          ; (fun _ => apply is_sized_pointer)
+          ; (fun _ => apply is_sized)
+          ; (fun _ => apply is_aggregate)
+          ; (fun _ => apply is_vector)
+          ; (fun _ => apply is_array)
+          ; (fun _ => apply is_struct)
+          ; (fun _ => apply x)
+          ; (fun _ => apply is_ptr_vector)
+          ; (fun _ => apply is_sized_ptr_vector)
+          ; (fun _ => apply is_sized_type_alias)
+          ; (fun _ => apply is_first_class_type)
+          ; (fun _ => apply is_function_pointer)
+        ];
+      apply w.
+  - apply is_non_void.
+Defined.
+
+Definition is_ptr_vector' {s : StorageType} : Lens' (Metadata s) (Component s Field unit).
+  red.
+  intros f F afa w.
+  refine open_constr:((fun x => _) <$> afa (_ w)); try typeclasses_eauto.
+  - apply mkMetadata;
+      Control.dispatch
+        [ (fun _ => apply name)
+          ; (fun _ => apply type_alias)
+          ; (fun _ => apply variable_type)
+          ; (fun _ => apply normalized_type)
+          ; (fun _ => apply is_local)
+          ; (fun _ => apply is_global)
+          ; (fun _ => apply is_deterministic)
+          ; (fun _ => apply is_non_deterministic)
+          ; (fun _ => apply from_pointer)
+          ; (fun _ => apply is_pointer)
+          ; (fun _ => apply is_sized_pointer)
+          ; (fun _ => apply is_sized)
+          ; (fun _ => apply is_aggregate)
+          ; (fun _ => apply is_vector)
+          ; (fun _ => apply is_array)
+          ; (fun _ => apply is_struct)
+          ; (fun _ => apply is_non_void)
+          ; (fun _ => apply x)
+          ; (fun _ => apply is_sized_ptr_vector)
+          ; (fun _ => apply is_sized_type_alias)
+          ; (fun _ => apply is_first_class_type)
+          ; (fun _ => apply is_function_pointer)
+        ];
+      apply w.
+  - apply is_ptr_vector.
+Defined.
+
+Definition is_sized_ptr_vector' {s : StorageType} : Lens' (Metadata s) (Component s Field unit).
+  red.
+  intros f F afa w.
+  refine open_constr:((fun x => _) <$> afa (_ w)); try typeclasses_eauto.
+  - apply mkMetadata;
+      Control.dispatch
+        [ (fun _ => apply name)
+          ; (fun _ => apply type_alias)
+          ; (fun _ => apply variable_type)
+          ; (fun _ => apply normalized_type)
+          ; (fun _ => apply is_local)
+          ; (fun _ => apply is_global)
+          ; (fun _ => apply is_deterministic)
+          ; (fun _ => apply is_non_deterministic)
+          ; (fun _ => apply from_pointer)
+          ; (fun _ => apply is_pointer)
+          ; (fun _ => apply is_sized_pointer)
+          ; (fun _ => apply is_sized)
+          ; (fun _ => apply is_aggregate)
+          ; (fun _ => apply is_vector)
+          ; (fun _ => apply is_array)
+          ; (fun _ => apply is_struct)
+          ; (fun _ => apply is_non_void)
+          ; (fun _ => apply is_ptr_vector)
+          ; (fun _ => apply x)
+          ; (fun _ => apply is_sized_type_alias)
+          ; (fun _ => apply is_first_class_type)
+          ; (fun _ => apply is_function_pointer)
+        ];
+      apply w.
+  - apply is_sized_ptr_vector.
+Defined.
+
+Definition is_sized_type_alias' {s : StorageType} : Lens' (Metadata s) (Component s Field unit).
+  red.
+  intros f F afa w.
+  refine open_constr:((fun x => _) <$> afa (_ w)); try typeclasses_eauto.
+  - apply mkMetadata;
+      Control.dispatch
+        [ (fun _ => apply name)
+          ; (fun _ => apply type_alias)
+          ; (fun _ => apply variable_type)
+          ; (fun _ => apply normalized_type)
+          ; (fun _ => apply is_local)
+          ; (fun _ => apply is_global)
+          ; (fun _ => apply is_deterministic)
+          ; (fun _ => apply is_non_deterministic)
+          ; (fun _ => apply from_pointer)
+          ; (fun _ => apply is_pointer)
+          ; (fun _ => apply is_sized_pointer)
+          ; (fun _ => apply is_sized)
+          ; (fun _ => apply is_aggregate)
+          ; (fun _ => apply is_vector)
+          ; (fun _ => apply is_array)
+          ; (fun _ => apply is_struct)
+          ; (fun _ => apply is_non_void)
+          ; (fun _ => apply is_ptr_vector)
+          ; (fun _ => apply is_sized_ptr_vector)
+          ; (fun _ => apply x)
+          ; (fun _ => apply is_first_class_type)
+          ; (fun _ => apply is_function_pointer)
+        ];
+      apply w.
+  - apply is_sized_type_alias.
+Defined.
+
+Definition is_first_class_type' {s : StorageType} : Lens' (Metadata s) (Component s Field unit).
+  red.
+  intros f F afa w.
+  refine open_constr:((fun x => _) <$> afa (_ w)); try typeclasses_eauto.
+  - apply mkMetadata;
+      Control.dispatch
+        [ (fun _ => apply name)
+          ; (fun _ => apply type_alias)
+          ; (fun _ => apply variable_type)
+          ; (fun _ => apply normalized_type)
+          ; (fun _ => apply is_local)
+          ; (fun _ => apply is_global)
+          ; (fun _ => apply is_deterministic)
+          ; (fun _ => apply is_non_deterministic)
+          ; (fun _ => apply from_pointer)
+          ; (fun _ => apply is_pointer)
+          ; (fun _ => apply is_sized_pointer)
+          ; (fun _ => apply is_sized)
+          ; (fun _ => apply is_aggregate)
+          ; (fun _ => apply is_vector)
+          ; (fun _ => apply is_array)
+          ; (fun _ => apply is_struct)
+          ; (fun _ => apply is_non_void)
+          ; (fun _ => apply is_ptr_vector)
+          ; (fun _ => apply is_sized_ptr_vector)
+          ; (fun _ => apply is_sized_type_alias)
+          ; (fun _ => apply x)
+          ; (fun _ => apply is_function_pointer)
+        ];
+      apply w.
+  - apply is_first_class_type.
+Defined.
+
+Definition is_function_pointer' {s : StorageType} : Lens' (Metadata s) (Component s Field unit).
+  red.
+  intros f F afa w.
+  refine open_constr:((fun x => _) <$> afa (_ w)); try typeclasses_eauto.
+  - apply mkMetadata;
+      Control.dispatch
+        [ (fun _ => apply name)
+          ; (fun _ => apply type_alias)
+          ; (fun _ => apply variable_type)
+          ; (fun _ => apply normalized_type)
+          ; (fun _ => apply is_local)
+          ; (fun _ => apply is_global)
+          ; (fun _ => apply is_deterministic)
+          ; (fun _ => apply is_non_deterministic)
+          ; (fun _ => apply from_pointer)
+          ; (fun _ => apply is_pointer)
+          ; (fun _ => apply is_sized_pointer)
+          ; (fun _ => apply is_sized)
+          ; (fun _ => apply is_aggregate)
+          ; (fun _ => apply is_vector)
+          ; (fun _ => apply is_array)
+          ; (fun _ => apply is_struct)
+          ; (fun _ => apply is_non_void)
+          ; (fun _ => apply is_ptr_vector)
+          ; (fun _ => apply is_sized_ptr_vector)
+          ; (fun _ => apply is_sized_type_alias)
+          ; (fun _ => apply is_first_class_type)
+          ; (fun _ => apply x)
+        ];
+      apply w.
+  - apply is_function_pointer.
+Defined.
+
+Definition ident_to_raw_id (i : ident) :=
+  match i with
+  | ID_Global id => id
+  | ID_Local id => id
+  end.
+
+Definition entl {m} `{HM: Monad m} (e : Ent) : Lens' (Metadata (WorldOf m)) (Metadata FieldOf).
+  red.
+  intros f F afa w.
+
+  refine
+    open_constr:
+      (let eid := unEnt e in
+       ((fun x => _) <$> afa (_ w))); try typeclasses_eauto.
+  - apply mkMetadata; red;
+      applyMetadataConstructors (fun _ => refine open_constr:(optSetMapRaw (_ x) eid (_ w))).
+  - intros w'.
+    apply (mkMetadata FieldOf);
+      refine open_constr:(IM.Raw.find eid (_ w'));
+      Control.dispatch metadataConstructors.
+Defined.
+
+Definition deleteEntity {w} {m} `{Monad m} `{@MetadataStore m Metadata (SystemState w m)} (e : Ent) : SystemT w m unit
+  := let eid := unEnt e in
+     metadata .@ entl e .= def;;
+     entities %= (fun ents => IS.remove eid ents);;
+     ret tt.
+
+Definition deleteEntities
+  {w : StorageType -> Type} {m : Type -> Type}
+  `{Monad m} `{@MetadataStore m Metadata (SystemState w m)} {A}
+  (es : IM.Raw.t A) : SystemT w m unit
+  := IM.Raw.fold (fun k _ acc => deleteEntity (mkEnt k);; acc) es (ret tt).
+
+Definition names'' {m} : Traversal (Metadata (WorldOf m)) (Metadata (WorldOf m)) (Component (WorldOf m) Field ident) (Component (WorldOf m) Field ident).
+  red.
+  intros f F focus meta.
+  refine open_constr:(pure (mkMetadata (WorldOf m)) <*> _ <*> _ <*> _ <*> _ <*> _ <*> _ <*> _
+                        <*> _ <*> _ <*> _ <*> _ <*> _ <*> _ <*> _ <*> _ <*> _ <*> _ <*> _
+                        <*> _ <*> _ <*> _ <*> _);
+    try typeclasses_eauto.
+  - apply (focus (name _ meta)).
+  - apply (pure (type_alias _ meta)).
+  - apply (pure (variable_type _ meta)).
+  - apply (pure (normalized_type _ meta)).
+  - apply (pure (is_local _ meta)).
+  - apply (pure (is_global _ meta)).
+  - apply (pure (is_deterministic _ meta)).
+  - apply (pure (is_non_deterministic _ meta)).
+  - apply (pure (from_pointer _ meta)).
+  - apply (pure (is_pointer _ meta)).
+  - apply (pure (is_sized_pointer _ meta)).
+  - apply (pure (is_sized _ meta)).
+  - apply (pure (is_aggregate _ meta)).
+  - apply (pure (is_vector _ meta)).
+  - apply (pure (is_array _ meta)).
+  - apply (pure (is_struct _ meta)).
+  - apply (pure (is_non_void _ meta)).
+  - apply (pure (is_ptr_vector _ meta)).
+  - apply (pure (is_sized_ptr_vector _ meta)).
+  - apply (pure (is_sized_type_alias _ meta)).
+  - apply (pure (is_first_class_type _ meta)).
+  - apply (pure (is_function_pointer _ meta)).
+Defined.
+
+Definition emap
+  {w m} `{Monad m} `{@MetadataStore m Metadata (SystemState w m)}
+  {es E} `{ToEnt E} `{Foldable es E}
+  (t : EntTarget w m (E:=E)) (q : QueryT Metadata m (Metadata SetterOf)) : SystemT w m unit
+  := es <- t;;
+     fold _
+       (fun (k : E) (acc : SystemT w m unit) =>
+          let e := toEnt k in
+          meta <- getEntity e;;
+          sets <- lift (unQueryT q e meta);;
+          match sets with
+          | None =>
+              acc
+          | Some s =>
+              setEntity e s;;
+              acc
+          end
+       ) (ret tt) es.
+
+(* Filter out Nones from a set of options *)
+Class FilterNone T :=
+  { filterNone : forall {a}, T (option a) -> T a }.
+
+#[global] Instance FilterNone_list : FilterNone list :=
+  { filterNone _ l := fold_right (fun x acc => match x with | None => acc | Some x => x :: acc end) [] l }.
+
+Program Definition efor
+  {w m} `{Monad m} `{@MetadataStore m Metadata (SystemState w m)}
+  {a}
+  (t : @EntTarget (list Ent) Ent _ _ w m) (q : QueryT Metadata m a) : SystemT w m (list a)
+  := es <- t;;
+     _.
+Next Obligation.
+  refine open_constr:(fmap filterNone _);
+    try typeclasses_eauto.
+  refine open_constr:((fun a b => mapT b a) es (fun e => cs <- getEntity (toEnt e);; lift (unQueryT q e cs)));
+    try typeclasses_eauto.
+Defined.
+
+Program Definition efind
+  {w m a} `{Monad m} `{@MetadataStore m Metadata (SystemState w m)}
+  {es E} `{ToEnt E} `{Foldable es E}
+  (t : EntTarget w m (E:=E))
+  (q : QueryT Metadata m a) : SystemT w m (option a)
+  := es <- t;;
+     _.
+Next Obligation.
+  refine
+    open_constr:
+      (fold _
+         (fun (k : E) (acc : SystemT w m (option a)) =>
+            let e := toEnt k in
+            meta <- getEntity e;;
+            qres <- lift (unQueryT q e meta);;
+            match qres with
+            | Some _ => ret qres
+            | None => acc
+            end
+         ) (ret None) es);
+    try typeclasses_eauto.
+Defined.
