src/coq/Utils/OptionUtil.v
@@ -1,3 +1,6 @@
+From ExtLib Require Import
+  Structures.Foldable.
+
 Definition guard_opt (x : bool) : option unit
   := if x then Some tt else None.
 
@@ -14,3 +17,16 @@ Definition option_rel2 {X1 X2 : Type} (R : X1 -> X2 -> Prop) : (option X1 -> opt
             | _, _ => False
             end.
 #[export] Hint Unfold option_rel2 : core.
+
+Import Monoid.
+#[global] Instance Foldable_option {a} : Foldable (option a) a.
+split.
+intros m M conv oa.
+apply (match oa with | Some a => conv a | None => (monoid_unit M) end).
+Defined.
+
+Definition maybe {a b} (def : b) (f : a -> b) (oa : option a) : b
+  := match oa with
+     | Some a => f a
+     | None => def
+     end.
